\documentclass{article}
\usepackage{amsmath}  % 数学符号包
\usepackage{amssymb}  % 更多数学符号
\usepackage{enumitem} % 列表样式
\usepackage{fancyhdr} % 页眉设置
\usepackage{geometry} % 页面设置
\usepackage[UTF8]{ctex}
\usepackage{bm}
\usepackage{amsthm}


\geometry{a4paper, margin=1in}


\pagestyle{fancy}
\fancyhf{}
\fancyhead[C]{Demo}
\fancyhead[R]{}


\title{Demo}
\author{noflowerzzk}
\date{}


\begin{document}
\maketitle

\section{$\mathcal{A} $}
已知$\displaystyle{\lim_{n \to \infty}x_n = A , y_n > 0, \lim_{n \to \infty}\frac{y_n}{y_1 + y_2 + \cdots + y_n} = 0}$ \\
证明: $\displaystyle{\lim_{n \to \infty}\frac{x_1 y_n + x_2 y_{n - 1} + \cdots + x_n y_1}{y_1 + y_2 + \cdots + y_n} = A}$.

\section{$\mathcal{B} $}
\[
\lim_{x \to 0}\frac{1 - \cos x \cos 2x \cdots \cos nx}{x^2}
= \lim_{x \to 0}\frac{\displaystyle{\sum_{k = 1}^{n}\cos x \cos 2x \cdots \sin kx \cdots \cos nx}}{2x}
= \frac{n(n + 1)}{4}
\]


\end{document}