\documentclass{article}
\usepackage{amsmath}  % 数学符号包
\usepackage{amssymb}  % 更多数学符号
\usepackage{enumitem} % 列表样式
\usepackage{fancyhdr} % 页眉设置
\usepackage{geometry} % 页面设置
% \usepackage[UTF8]{ctex}
\usepackage{bm}
\usepackage{amsthm}
\everymath{\displaystyle}  % 让所有数学模式都使用 \displaystyle
\newcommand{\lb}{\left\llbracket}
\newcommand{\rb}{\right\rrbracket}


\geometry{a4paper, margin=1in}


\pagestyle{fancy}
\fancyhf{}
\fancyhead[C]{Discrete Math Homework 11}
\fancyhead[R]{2024.11.20}

\title{Discrete Math Homework 11}
\author{noflowerzzk}
\date{2024.11.20}


\begin{document}
\maketitle

\section{}

Let $A = [0, 1], B = (0, 1)$, then $C_0 = A \setminus \left\{G(b) | b \in B\right\} = \left\{0, 1\right\}$, $D_0 = \left\{F(a) | a \in C_0 \right\} = \left\{\frac{1}{3}, \frac{2}{3}\right\}$. \\
According to the define, 
\[
    C_{n + 1} = \left\{G(b) | b \in D_n\right\} = \left\{G(F(a)) | a \in C_n\right\} = \left\{\frac{1}{3}x +\frac{1}{3} | x \in C_n\right\}
\]
Then we have $C_n = \left\{\frac{1}{2} - \frac{1}{2}\cdot \frac{1}{3^n}, \frac{1}{2} + \frac{1}{2}\cdot \frac{1}{3^n}\right\}$, $D_n = \left\{\frac{1}{2} - \frac{1}{2}\cdot \frac{1}{3^{n + 1}}, \frac{1}{2} + \frac{1}{2}\cdot \frac{1}{3^{n + 1}}\right\} = C_{n + 1}$ \\
Let $H: A \to B$, 
\[H(a) = \begin{cases}
    \frac{1}{3}a + \frac{1}{3}, & \quad a \in \bigcup_{n = 0}^{\infty}C_n \\
    a, & \quad a \notin \bigcup_{n = 0}^{\infty}C_n
\end{cases}\]
obviously $H$ is a function. \\
$\forall b \in D_n$, $\exists a \in C_n, F(a) = b$. $\forall b \in B \setminus \bigcup_{n = 0}^{\infty}D_n, H(b) = b$, because if $a \in C_i$, then $b = H(a) \in D_i$, contradicts with $b \in B \setminus \bigcup_{n = 0}^{\infty}D_n$. So $H$ is surjective. \\
If $a, a' \in \bigcup_{n = 0}^{\infty}C_n$, then $H(a), H(a') \in \bigcup_{n = 0}^{\infty}D_n$. If $H(a) = H(a') \in D_n$, then $\frac{1}{3}a + \frac{1}{3} = \frac{1}{3}a' + \frac{1}{3} \Rightarrow a = a'$.
If $a, a' \notin \bigcup_{n = 0}^{\infty}C_n$, if $H(a) = H(a')$, then $a = a'$. So $H$ is injective. \\
So $H$ is a bijection from $[0, 1]$ to $(0, 1)$.

\section{}

\begin{itemize}
    \item [a)]
    \begin{proof}
        If $\left(a, [a]_R\right), \left(a, [a']_R\right)$, then $a = a = a'$, so $F$ is a function.
    \end{proof}
    \item [b)] 
    \begin{proof}
        $\forall b = [a]_R \in B$, $\exists a \in A, F(a) = [a]_R$, so $F$ is a surjection from $A$ to $B$.
    \end{proof}
    \item [c)]
    \begin{proof}
        For any $(a, b) \in \left\{(a, b) | F(a) = F(b)\right\}$, we have $[a]_R = [b]_R$, i.e. $(a, b) \in R$, $\left\{(a, b) | F(a) = F(b)\right\} \subseteq R$. \\
        For any $(a, b) \in R$, we have $[a]_R = [b]_R$, so $F(a) = F(b)$, $(a, b) \in \left\{(a, b) | F(a) = F(b)\right\}$, $R \subseteq \left\{(a, b) | F(a) = F(b)\right\}$. \\
        In summary, $R =  \left\{(a, b) | F(a) = F(b)\right\}$
    \end{proof}
\end{itemize}

\section{}

\begin{itemize}
    \item
    \begin{proof}
        According to $aR_1a, bR_2b$, $((a, b), (a, b)) \in R$, $R$ is reflexive. \\
        According to $aR_1b, bR_1c \Rightarrow aR_1c$, $a'R_2b', b'R_2c' \Rightarrow a'R_2c'$, then $((a, a'), (b, b')) \in R$, $((b, b'), (c, c')) \in R$, then $((a, a'), (c, c')) \in R$, $R$ is transitive. \\
        According to $aR_1a' \Leftrightarrow a'R_1a$, $bR_2b' \Leftrightarrow b'R_2b$, we have $((a, b), (a', b')) \in R \Leftrightarrow ((a', b'), (a, b)) \in R$, $R$ is symmetric. \\
        In summary, $R$ is a equivalence relations on $A_1 \times A_2$.
    \end{proof} 
    \item 
    \begin{proof}
        Let $F \subseteq (P_1 \times P_2) \times P$, $\forall a_1 \in A_1, a_2 \in A_2$, $\left(([a_1]_{R_1}, [a_2]_{R_2}), [(a_1, a_2)]_R\right) \in F$. Now we prove that $F$ is a bijection from $P_1 \times P_2$ to $P$. \\
        According to $F$'s definition, $F$ is a function. \\
        $\forall [(a_1, a_2)]_R \in P$, there exists $([a_1]_{R_1}, [a_2]_{R_2}) \in P_1 \times P_2$, $F(([a_1]_{R_1}, [a_2]_{R_2})) = [(a_1, a_2)]_R$, $F$ is a injection. \\
        If $F(([a]_{R_1}, [b]_{R_2})) = F(([a']_{R_1}, [b']_{R_2})) = [(a_0, b_0)]_R$, then $[(a, b)]_R = [(a', b')]_R = [(a_0, b_0)]_R$, so $((a, b), (a', b')) \in R$, i,e, $aR_1a', bR_2b'$, so $[a]_{R_1} = [a']_{R_1}, [b]_{R_2} = [b']_{R_2}$, $([a]_{R_1}, [b]_{R_2}) = ([a']_{R_1}, [b']_{R_2})$, $F$ is a surjection. \\
        So $F$ is a bijection, so $P_1 \times P_2 \approx P$.
    \end{proof}
\end{itemize}

\end{document}