\special{dvipdfmx:config z 0} %取消PDF压缩，加快速度，最终版本生成的时候最好把这句话注释掉

\documentclass{ctexart}
\usepackage{newtxtext, geometry, amsmath, amssymb}
\usepackage{stmaryrd}
\usepackage{amsthm} % 设置定理环境，要在amsmath后用
\usepackage{xpatch} % 用于去除amsthm定义的编号后面的点
\usepackage[strict]{changepage} % 提供一个 adjustwidth 环境
\usepackage{multicol} % 用于分栏
\usepackage[fontsize=14pt]{fontsize} % 字号设置
\usepackage{esvect} % 实现向量箭头输入（显示效果好于\vec{}和\overrightarrow{}），格式为\vv{⟨向量符号⟩}或\vv*{⟨向量符号⟩}{⟨下标⟩} 
\usepackage[
            colorlinks, % 超链接以颜色来标识，而并非使用默认的方框来标识
            linkcolor=mlv,
            anchorcolor=mlv,
            citecolor=mlv % 设置各种超链接的颜色
            ]
            {hyperref} % 实现引用超链接功能
\usepackage{tcolorbox} % 盒子效果
\usepackage{hyperref}
\tcbuselibrary{most} % tcolorbox宏包的设置，详见宏包说明文档

\geometry{a4paper,centering,scale=0.8}

% ————————————————————————————————————自定义符号————————————————————————————————————
\newcommand{\。}{．} % 示例：将指令\。定义为全角句点。
\newcommand{\zte}{\mathrm{e}} % 正体e
\newcommand{\ztd}{\mathrm{d}} % 正体d
\newcommand{\zti}{\mathrm{i}} % 正体i
\newcommand{\ztj}{\mathrm{j}} % 正体j
\newcommand{\ztk}{\mathrm{k}} % 正体k
\newcommand{\CC}{\mathbb{C}} % 黑板粗体C
\newcommand{\QQ}{\mathbb{Q}} % 黑板粗体Q
\newcommand{\RR}{\mathbb{R}} % 黑板粗体R
\newcommand{\ZZ}{\mathbb{Z}} % 黑板粗体Z
\newcommand{\NN}{\mathbb{N}} % 黑板粗体N
\newcommand{\lb}{\left\llbracket}
\newcommand{\rb}{\right\rrbracket}
% ————————————————————————————————————自定义符号————————————————————————————————————

% ————————————————————————————————————自定义颜色————————————————————————————————————
\definecolor{mlv}{RGB}{40, 137, 124} % 墨绿
\definecolor{qlv}{RGB}{240, 251, 248} % 浅绿
\definecolor{slv}{RGB}{33, 96, 92} % 深绿
\definecolor{qlan}{RGB}{239, 249, 251} % 浅蓝
\definecolor{slan}{RGB}{3, 92, 127} % 深蓝
\definecolor{hlan}{RGB}{82, 137, 168} % 灰蓝
\definecolor{qhuang}{RGB}{246, 250, 235} % 浅黄
\definecolor{shuang}{RGB}{77, 82, 59} % 深黄
\definecolor{qzi}{RGB}{240, 243, 252} % 浅紫
\definecolor{szi}{RGB}{49, 55, 70} % 深紫
% 将RGB换为rgb，颜色数值取值范围改为0到1
% ————————————————————————————————————自定义颜色————————————————————————————————————

% ————————————————————————————————————盒子设置————————————————————————————————————
% tolorbox提供了tcolorbox环境，其格式如下：
% 第一种格式：\begin{tcolorbox}[colback=⟨背景色⟩, colframe=⟨框线色⟩, arc=⟨转角弧度半径⟩, boxrule=⟨框线粗⟩]   \end{tcolorbox}
% 其中设置arc=0mm可得到直角；boxrule可换为toprule/bottomrule/leftrule/rightrule可分别设置对应边宽度，但是设置为0mm时仍有细边，若要绘制单边框线推荐使用第二种格式
% 方括号内加上title=⟨标题⟩, titlerule=⟨标题背景线粗⟩, colbacktitle=⟨标题背景线色⟩可为盒子加上标题及其背景线
\newenvironment{kuang1}{
    \begin{tcolorbox}[colback=hlan, colframe=hlan, arc = 1mm]
    }
    {\end{tcolorbox}}
\newenvironment{kuang2}{
    \begin{tcolorbox}[colback=hlan!5!white, colframe=hlan, arc = 1mm]
    }
    {\end{tcolorbox}}
% 第二种格式：\begin{tcolorbox}[enhanced, colback=⟨背景色⟩, boxrule=0pt, frame hidden, borderline={⟨框线粗⟩}{⟨偏移量⟩}{⟨框线色⟩}]   {\end{tcolorbox}}
% 将borderline换为borderline east/borderline west/borderline north/borderline south可分别为四边添加框线，同一边可以添加多条
% 偏移量为正值时，框线向盒子内部移动相应距离，负值反之
\newenvironment{kuang3}{
    \begin{tcolorbox}[enhanced, breakable, colback=hlan!5!white, boxrule=0pt, frame hidden,
        borderline south={0.5mm}{0.1mm}{hlan}]
    }
    {\end{tcolorbox}}
\newenvironment{lvse}{
    \begin{tcolorbox}[enhanced, breakable, colback=qlv, boxrule=0pt, frame hidden,
        borderline west={0.7mm}{0.1mm}{slv}]
    }
    {\end{tcolorbox}}
\newenvironment{lanse}{
    \begin{tcolorbox}[enhanced, breakable, colback=qlan, boxrule=0pt, frame hidden,
        borderline west={0.7mm}{0.1mm}{slan}]
    }
    {\end{tcolorbox}}
\newenvironment{huangse}{
    \begin{tcolorbox}[enhanced, breakable, colback=qhuang, boxrule=0pt, frame hidden,
        borderline west={0.7mm}{0.1mm}{shuang}]
    }
    {\end{tcolorbox}}
\newenvironment{zise}{
    \begin{tcolorbox}[enhanced, breakable, colback=qzi, boxrule=0pt, frame hidden,
        borderline west={0.7mm}{0.1mm}{szi}]
    }
    {\end{tcolorbox}}
% tcolorbox宏包还提供了\tcbox指令，用于生成行内盒子，可制作高光效果
\newcommand{\hl}[1]{
    \tcbox[on line, arc=0pt, colback=hlan!5!white, colframe=hlan!5!white, boxsep=1pt, left=1pt, right=1pt, top=1.5pt, bottom=1.5pt, boxrule=0pt]
{\bfseries \color{hlan}#1}}
% 其中on line将盒子放置在本行（缺失会跳到下一行），boxsep用于控制文本内容和边框的距离，left、right、top、bottom则分别在boxsep的参数的基础上分别控制四边距离
% ————————————————————————————————————盒子设置————————————————————————————————————

% ————————————————————————————————————自定义字体设置————————————————————————————————————
\setCJKfamilyfont{xbsong}{方正小标宋简体}
\newcommand{\xbsong}{\CJKfamily{xbsong}}
% CTeX宏集还预定义了\songti、\heiti、\fangsong、\kaishu、\lishu、\youyuan、\yahei、\pingfang等字体命令
% 由于未知原因，一些设备可能无法调用这些字体，故此文档暂时未使用
% ————————————————————————————————————自定义字体设置————————————————————————————————————

% ————————————————————————————————————各级标题设置————————————————————————————————————
\ctexset{
    % 修改 section。
    section={   
    % 设置标题编号前后的词语，使用name={⟨前部分⟩,⟨后部分⟩}参数进行设置。    
        name={\textbf{Chapter}\hspace{6pt} , \hspace{6pt}},
    % 使用number参数设置标题编号，\arabic设置为阿拉伯数字，\chinese设置为中文，\roman设置为小写罗马字母，\Roman设置为大写罗马字母，\alph设置为小写英文，\Alph设置为大写英文。
        number={\textbf{\Roman{section}}},
    % 参数format设置标题整体的样式。包括标题主题、编号以及编号前后的词语。
    % 参数format还可以设置标题的对齐方式。居中对齐\centering，左对齐\raggedright，右对齐\hfill
        format=\color{hlan}\centering\zihao{2}, % 设置 section 标题为正蓝色、黑体、居中对齐、小二号字
    % 取消编号后的空白。编号后有一段空白，参数aftername=\hspace{0pt}可以用来控制编号与标题之间的距离。
        aftername={}
    },
    % 修改 subsection。
    subsection={   
        name={\S \hspace{6pt}\hspace{8pt}},
        number={\arabic{section}.\arabic{subsection}\hspace{5pt}},
        format=\color{hlan}\centering\zihao{-2}, % 设置 subsection 标题为黑体、三号字
        aftername=\hspace{0pt}
    },
    subsubsection={   
        name={ , \hspace{3pt}},
        number={\arabic{subsubsection}},
        format=\raggedright\color{hlan}\zihao{3},
        aftername=\hspace{0pt}
    },
    part={   
        name={Part\hspace{2pt} , },
        number={\Roman{part}},
        format=\color{white}\centering\bfseries\zihao{-1},
        aftername=\hspace{1em}
    }
}
% 各个标题设置的各行结尾一定要记得写逗号！！！！！！！！！！！！！！！！！！！！！！！！！！！！！！！！！！！！！！！！！！
% ————————————————————————————————————各级标题设置————————————————————————————————————

% ————————————————————————————————————定理类环境设置————————————————————————————————————
\newtheoremstyle{t}{0pt}{}{}{\parindent}{\bfseries}{}{1em}{} % 定义新定理风格。格式如下：
%\newtheoremstyle{⟨风格名⟩}
%                {⟨上方间距⟩} % 若留空，则使用默认值
%                {⟨下方间距⟩} % 若留空，则使用默认值
%                {⟨主体字体⟩} % 如 \itshape
%                {⟨缩进长度⟩} % 若留空，则无缩进；可以使用 \parindent 进行正常段落缩进
%                {⟨定理头字体⟩} % 如 \bfseries
%                {⟨定理头后的标点符号⟩} % 如点号、冒号
%                {⟨定理头后的间距⟩} % 不可留空，若设置为 { }，则表示正常词间间距；若设置为 {\newline}，则环境内容开启新行
%                {⟨定理头格式指定⟩} % 一般留空
% 定理风格决定着由 \newtheorem 定义的环境的具体格式，有三种定理风格是预定义的，它们分别是：
% plain: 环境内容使用意大利斜体，环境上下方添加额外间距
% definition: 环境内容使用罗马正体，环境上下方添加额外间距
% remark: 环境内容使用罗马正体，环境上下方不添加额外间距
\theoremstyle{t} % 设置定理风格
\newtheorem{dyhj}{\color{slv} Definition}[subsection] % 定义定义环境，格式为\newtheorem{⟨环境名⟩}{⟨定理头文本⟩}[⟨上级计数器⟩]或\newtheorem{⟨环境名⟩}[⟨共享计数器⟩]{⟨定理头文本⟩}，其变体\newtheorem*不带编号
\newtheorem{dlhj}{\color{shuang} Theorem}[subsection]
\newtheorem{lthj}{\color{szi} Example}[subsection]
\newtheorem*{jiehj}{\color{slan} Solve}
\newtheorem*{zmhj}{\color{slan} Proof}
\newenvironment{dy}{\begin{lvse}\begin{dyhj}}{\end{dyhj}\end{lvse}}
\newenvironment{zm}{\begin{lanse}\begin{zmhj}}{$\hfill \square$\end{zmhj}\end{lanse}}
\newenvironment{dl}{\begin{huangse}\begin{dlhj}}{\end{dlhj}\end{huangse}}
\newenvironment{lt}{\begin{zise}\begin{lthj}}{\end{lthj}\end{zise}}
% ————————————————————————————————————定理类环境设置————————————————————————————————————

% ————————————————————————————————————目录设置————————————————————————————————————
\setcounter{tocdepth}{4} % 设置在 ToC 的显示的章节深度
\setcounter{secnumdepth}{3} % 设置章节的编号深度
% 数值可选选项：-1 part 0 chapter 1 section 2 subsection 3 subsubsection 4 paragraph 5 subparagraph
\renewcommand{\contentsname}{Contents}
% ————————————————————————————————————目录设置————————————————————————————————————

\everymath{\displaystyle} % 设置所有数学公式显示为行间公式的样式

\begin{document}

\quad\\
{
\Huge \bfseries 
\begin{kuang3}
    \color{hlan}
    \centering
    Discrete Math
\end{kuang3}
}

\thispagestyle{empty} % 取消这一页的页码
\newpage

% ————————————————————————————————————页码设置————————————————————————————————————
\pagenumbering{Roman}
\setcounter{page}{1}

\begin{multicols}{2} % 设置环境中内容为两栏。数字为栏数
    {
    \tableofcontents
    }
\end{multicols}

\newpage
\setcounter{page}{1}
\pagenumbering{arabic}
% ————————————————————————————————————页码设置————————————————————————————————————

% 指令\addcontentsline{toc}{⟨章节层级⟩}{⟨标题名⟩}可将“⟨标题名⟩”加入目录。如为无章节层级的标题，可先用\phantomsection指令添加section分级

\begin{kuang1}
    \part{Discrete Math: Logic}
\end{kuang1}

\begin{kuang2}
    \section{Propositional Logic}
\end{kuang2}

\begin{kuang3}
    \subsection{Connectives and Truth Assingments}
\end{kuang3}


\begin{dy} % 开始定义环境，格式为\begin{⟨环境名⟩}[⟨定理名⟩]
[Truth table of Connectives](Omitted)
\end{dy}

\begin{dy}[Truth Assingments] 
    Suppose $\Sigma $ is the set of propositional variables. A mapping from $\Sigma$ to $\{\mathbf{T}, \mathbf{F}\}$ called a truth assignment.
\end{dy}

\begin{dy}
    Suppose $\Sigma $ is the set of propositional variables and $\mathcal{J}: \Sigma \rightarrow \{\mathbf{T}, \mathbf{F}\}$ is a truth assignment. The truth value of the compond proposition on $\mathcal{J}$ \dots \\ (Omitted)
\end{dy}

\begin{dy}[Tautology, contradiction]
    (Omitted)
\end{dy}

\begin{dy}[Contingency, Satisfiable]
    A \textcolor{shuang}{contingency} is a compound proposition that is neither a tautology nor a contradiction. \\
    A compound proposition is \textcolor{shuang}{satisfiable} if it is true under some truth assignment.
\end{dy}

\begin{kuang3}
    \subsection{Consequence and Equivalent}
\end{kuang3}

\subsubsection{The definition of consequence and logically equivalent}

\begin{dy}[Consequence]
    Suppose $\Phi$ is a set of propositions and $\psi$ is one single proposition. We say that $\psi$ is a consequence of $\Phi$, written as $\Phi \models \psi$. if $\Phi$ 's being all true implies that $\psi$ is also true. \\
    In other words, $\Phi \models \psi$ if for any truth assignment $\mathcal{J}, \llbracket \phi \rrbracket_{\mathcal{J}}=\mathbf{T}$ for any $\phi \in \Phi$ implies $\llbracket \psi \rrbracket_{\mathcal{J}}=\mathbf{T}$.
\end{dy}

\begin{dy}[Logically Equivalent]
    $\phi$ is a logically equivalent to $\psi$, written as $\phi \equiv \psi$, if $\phi$ 's truth value and $\psi$ 's truth value are the same under any situation. In other words, $\phi \equiv \psi$ if $\llbracket \phi \rrbracket_{\mathcal{J}}=\llbracket \psi \rrbracket_{\mathcal{J}}$ for any truth assignment $\mathcal{J}$.
\end{dy}

\begin{lt}
    $\Phi = \{\ \}$, $\psi = p \lor \lnot p$, $\Phi \models \psi$
\end{lt}

\subsubsection{Important properties}

\begin{dl} \quad 
    \begin{itemize}
        \item $\phi \lor \lnot \phi$ is an tautology 
        \item $\phi \land \lnot \phi$ is a contradiction 
        \item $\phi, \psi \models \phi \land \psi$ ($\land$-Introduction)
        \item $\phi \land \psi \models \phi$ ($\land$-Elimination)
        \item $\phi \models \phi \lor \psi$ ($\lor$-Introduction)
        \item If $\Phi, \phi_1 \models \psi, \Phi, \phi_2 \models \psi$, then $\Phi, \phi_1 \lor \phi_2 \models \psi$ ($\lor$-Elimination)
    \end{itemize}
    \begin{zmhj}[Proof of the last one]
        Suppose $\lb \phi \rb_\mathcal{J} = \mathbf{T}$, $\lb \phi_1 \lor \phi_2\rb_\mathcal{J} = \mathbf{T}$. \\
        Then at least one of the following holds: $\lb \phi_1\rb_\mathcal{J} = \mathbf{T}, \lb \phi_2\rb_\mathcal{J} = \mathbf{T}$.
        \qed
    \end{zmhj}
\end{dl}

\begin{dl}[Contrapositive]
    If $\Phi, \lnot \phi \models \psi$, then $\Phi, \lnot \psi \models \phi$ 
\end{dl}

\begin{dl} \quad
    \begin{itemize}
        \item $\lnot (\lnot q) \equiv q$ \quad (Double Negation)
        \item $\phi \land \phi \equiv \phi, \quad \phi \lor \phi \equiv \phi$ \quad (Idempotent Laws)
        \item $\phi \land \psi \equiv \psi \land \psi, \quad \phi \lor \psi \equiv \psi \lor \psi$ \quad (Commutative Laws)
        \item $\phi \lor (\psi \land \chi) \equiv (\phi \lor \psi) \land (\phi \lor \chi), \quad \phi \land (\psi \lor \chi) \equiv (\phi \land \psi) \lor (\phi \land \chi)$ \quad (Distributive Laws)
        \item $\lnot (q \land q) \equiv \lnot p \lor \lnot q, \quad \lnot (q \lor q) \equiv \lnot p \land \lnot q$ \quad (De Morgan's Laws)
        \item $\phi \land (\lnot \phi) \equiv \mathbf{F}$, \quad $\phi \lor (\lnot\phi) \equiv \mathbf{T}$ \quad (Negation Laws)
        \item $\phi \land \mathbf{T} \equiv \phi, \quad \phi \lor \mathbf{F} \equiv \phi, \quad \phi \land \mathbf{F} \equiv \mathbf{F}, \quad \phi \lor \mathbf{T} \equiv \mathbf{T}$ \quad (Laws of logical constants)
        \item $\phi \lor (\phi \land \psi) \equiv \phi, \quad \phi \land (\phi \lor \psi) \equiv \phi$ \quad (Absorption Laws)
    \end{itemize}
\end{dl}

\subsubsection{Prove Logical Equivalence}

\begin{dl}[Transitivity]
    If $\phi \equiv \psi$ and $\psi \equiv \chi$, then $\phi \equiv \chi$.
\end{dl}

\begin{dl}[Congruence Property] \quad 
    \begin{itemize} 
        \item If $\phi \equiv \psi$, then $\lnot\phi \equiv \lnot\psi$
        \item If $\phi_1 \equiv \phi_2$, $\psi_1 \equiv \psi_2$, then $\phi_1 \land \psi_1 \equiv \phi_2 \land \psi_2$
        \item If $\phi_1 \equiv \phi_2$, $\psi_1 \equiv \psi_2$, then $\phi_1 \lor \psi_1 \equiv \phi_2 \lor \psi_2$
    \end{itemize}
\end{dl}

\begin{dl}[Reflexivity]
    $\phi \equiv \phi$
\end{dl}

\subsubsection{Relation among tautologies, contradictions, satisfiable assertions, consequence relations and logic equivalence}

\begin{dl} \quad 
    \begin{itemize}
        \item $\phi_1, \phi_2, \cdots \phi_n \models \psi$ iff. $\left(\bigwedge _{k = 1}^n\phi_i\right) \land \lnot \psi$ is not satisfiable.
        \item $\{\ \} \models \phi$ iff. $\phi$ is an tautology.
        \item $\phi \equiv \psi$ iff. $\phi \models \psi$ and $\psi \models \phi$.
    \end{itemize}
\end{dl}

\begin{dl}
    If $\phi \models \psi$ and $\psi \models \chi$, then $\phi \models \chi$.
\end{dl}

\begin{kuang3}
    \subsection{Normal Forms}
\end{kuang3}

\begin{dy}[Disjunctive Normal Form,\ DNF] \quad 
    \begin{itemize}
        \item A \textcolor{shuang}{\textbf{literal}} is a propositional variable or its negation.
        \item A \textcolor{shuang}{\textbf{conjunctive clause}} is a conjunctions of literals.
        \item A \textcolor{shuang}{\textbf{compound proposition}} is in disjunctive normal form if it is a disjunction of conjunctive clauses.
    \end{itemize}
\end{dy}

\begin{dy}[Conjunctive Normal Form, \  CNF] \quad \\
    (Similar as above)
\end{dy}

\begin{lt} \quad
    \begin{itemize}
        \item literals $x, y, z, p, q, r, \lnot q$
        \item conjunctive clauses $p, p \land q, \lnot p \land q$
        \item DNF $p, p \lor (\lnot q \land r), \lnot p \lor (q \land p \land r)$
    \end{itemize}
\end{lt}

\begin{dl}
    Every compound proposition is logically equivalent to some compound proposition in DNF.
    \begin{zmhj}[Proof 1]
        Suppose that the compound proposition $\phi$ consists of the literals $p_1, p_2, \cdots, p_n$. \\
        For all $\mathcal{J}$ as a interpretation, we only need to prove that 
        \[
            \phi \equiv \bigvee_{\lb \phi \rb_\mathcal{J} = \mathbf{T}}\left(\bigwedge_{\mathcal{J}(p_i) = \mathbf{T}}p_i \land \bigwedge_{\mathcal{J}(p_i) = \mathbf{F}}\lnot p_i \right)
        \]
        Consider a specific interpretation $\mathcal{J}_0$, if $\lb \phi\rb_\mathcal{J} = \mathbf{T}$, then
        \[
            \left\llbracket \bigvee_{\lb \phi \rb_\mathcal{J} = \mathbf{T}}\left(\bigwedge_{\mathcal{J}(p_i) = \mathbf{T}}p_i \land \bigwedge_{\mathcal{J}(p_i) = \mathbf{F}}\lnot p_i \right) \right\rrbracket_{\mathcal{J}_0} 
             = \lb \left(\bigwedge_{\mathcal{J}_0(p_i) = \mathbf{T}}p_i \land \bigwedge_{\mathcal{J}_0(p_i) = \mathbf{F}}\lnot p_i\right)\rb_{\mathcal{J}_0} 
        \]
        If $\mathcal{J}_0(p_i) = \mathbf{T}$, then $\lb p_i \rb_{\mathcal{J_0}} = \mathbf{T}$, \\
        if $\mathcal{J}_0(p_i) = \mathbf{F}$, then $\lb \lnot p_i \rb_{\mathcal{J_0}} = \mathbf{T}$. \\
        So
        \[
            \lb \left(\bigwedge_{\mathcal{J}_0(p_i) = \mathbf{T}}p_i \land \bigwedge_{\mathcal{J}_0(p_i) = \mathbf{F}}\lnot p_i\right)\rb_{\mathcal{J}_0} = \mathbf{T}
        \]
        \qed
    \end{zmhj}
    \begin{zmhj}[Proof 2]
        Define $DNF(\phi)$ as follow and prove that $DNF(\phi) \equiv \phi$. 
        \begin{dyhj}
            \begin{itemize}
                \item $DNF(\phi) \triangleq DNF_2(DNF_1(\phi))$
                \item 
                    $DNF_1(\lnot \lnot \phi) = DNF_1(\phi)$. \\
                    (The De Morgan's law) \\
                    $DNF_1(\phi \land \psi) = DNF_1(\phi) \land DNF_1(\psi)$ \quad ($\lor$ is the same) \\
                    $DNF_1(l) = l$ \quad $l$ is a literal.
                \item 
                    $DNF_2(l) = l$ \quad $l$ is a literal, \\
                    $DNF_2(\phi \lor \psi) = DNF_2(\phi) \lor DNF_2(\psi)$ \\
                    If $\phi = \bigvee_{i = 1}^{n}\phi_i, \psi = \bigvee_{j = 1}^{m}\psi_j$, then 
                    \[
                        DNF_2(\phi \land \psi) = \bigvee_{i = 1}^{n}\bigvee_{j = 1}^{m}(\phi_i \land \psi_j)
                    \]
                \end{itemize}
        \end{dyhj}
        Then it's obvious that $\phi \equiv DNF(\phi)$ and $DNF(\phi)$ is a DNF. 
        \qed
    \end{zmhj}
\end{dl}

\begin{dl}
    Every compound proposition is logically equivalent to some compound proposition in CNF.
    \begin{zmhj}
        (Similar as above)
    \end{zmhj}
\end{dl}

\begin{lt}[*]
    The CDCL algorithm. \\
    (Suspended now)
\end{lt}

\begin{kuang2}
    \section{First Order Logic, \ FOL}
\end{kuang2}

\begin{kuang3}
    \subsection{The syntax of first order language}
\end{kuang3}

\begin{dy} \quad
    \begin{itemize}
        \item Predicate Logic's Language
        \begin{itemize}
            \item Variables $x, y, z, \cdots$
            \item Constants $c_1, c_2, \cdots$
            \item Prelicates $P, Q, R, \cdots$
            \item Functions $f, g, h, \cdots$
            \item Logic patterns $\exists, \forall, \land, \lor, \lnot$
        \end{itemize}
        \item Terms $x, y, c_1, c_2, f(x), g(x, y), \cdots$
        \item propositions $P(x), Q(f(x, g(x, y))), \exists x \forall y R(x, g(y)), \cdots$
    \end{itemize}
\end{dy}

\begin{kuang3}
    \subsection{The semantics of first order language}
\end{kuang3}

\subsubsection{Structure}

\begin{dy}[$S$-structure]\quad \\
    Given a sumbol set $S$, an $S$-structure $\mathcal{A} = \left(A, \alpha\right)$ contains
    \begin{itemize}
        \item a domain $A$, which is a non-empty set.
        \item an interpretation of every predicate symbol.
        \begin{lthj}
            if $P$ is a symbol of binary predicate, then $\alpha(P)$ is a mapping from $A \times A$ to $\{\mathbf{T}, \mathbf{F}\}$.
        \end{lthj}
        \item an interpretation of every function symbol.
        \begin{lthj}
            if $f$ is a symbol of unary function, then $\alpha(f)$ is a mapping from $A$ to $A$.
        \end{lthj}
        \item an interpretation of every constant symbol.
        \begin{lthj}
            if $s$ is a constant symbol, $\alpha(c)$ is an element in domain $A$.
        \end{lthj}
    \end{itemize}
\end{dy}

With a structure, we can determine the truth of an closed proposition.

\subsubsection{Interpretation}

\begin{dy}[$S$-interpretation]\quad \\
    Given a symbol set $S$, a $S$-interpretation $\mathcal{J} = (\mathcal{A}, \beta)$ is
    \begin{itemize}
        \item a \( S \)-structure \( \mathcal{A} = (A, \alpha) \)
        \item a \( S \)-assignment \( \beta \): a mapping from variables to elements in the domain \( A \)
    \end{itemize}
        
    For \( \mathcal{J} = (\mathcal{A}, \beta) \) and \( \mathcal{A} = (A, \alpha) \), we usually use \( \mathcal{J}(P) \) and \( \mathcal{A}(P) \) to represent \( \alpha(P) \), use \( \mathcal{J}(f) \) and \( \mathcal{A}(f) \) to represent \( \alpha(f) \), use \( \mathcal{J}(c) \) and \( \mathcal{A}(c) \) to represent \( \alpha(c) \), and use \( \mathcal{J}(x) \) to represent \( \beta(x) \).        
\end{dy}

\begin{dy}[Terms' denotation]\quad \\
    For $S$-interpretation $\mathcal{J}$ and a $S$-term $t$,
    \begin{itemize}
        \item $\llbracket x \rrbracket_{\mathcal{J}} = \mathcal{J}(x)$
        \item $\llbracket c \rrbracket_{\mathcal{J}} = \mathcal{J}(c)$
        \item $\llbracket f(t_1, t_2, \dots, t_n) \rrbracket_{\mathcal{J}} = \mathcal{J}(f) \big( \llbracket t_1 \rrbracket_{\mathcal{J}}, \llbracket t_2 \rrbracket_{\mathcal{J}}, \dots, \llbracket t_n \rrbracket_{\mathcal{J}} \big)$
    \end{itemize}
\end{dy}

\begin{dy}[Propositions' truth]\quad \\
    For $S$-interpretation $\mathcal{J}$ and a $S$-proposition $t$,
    \begin{itemize}
        \item $\llbracket P(t_1, t_2, \dots, t_n) \rrbracket_{\mathcal{J}} = \mathcal{J}(P) \big( \llbracket t_1 \rrbracket_{\mathcal{J}}, \llbracket t_2 \rrbracket_{\mathcal{J}}, \dots, \llbracket t_n \rrbracket_{\mathcal{J}} \big)$
        \item $\llbracket \varphi \land \psi \rrbracket_{\mathcal{J}} = \llbracket \land \rrbracket \big( \llbracket \varphi \rrbracket_{\mathcal{J}}, \llbracket \psi \rrbracket_{\mathcal{J}} \big)$
        \item $\llbracket \neg \varphi \rrbracket_{\mathcal{J}} = \llbracket \neg \rrbracket \big( \llbracket \varphi \rrbracket_{\mathcal{J}} \big)$
        \item $\llbracket \forall x \varphi \rrbracket_{\mathcal{J}} = \mathbf{T}$ if and only if for every $a$ in $\mathcal{A}$'s domain, $\llbracket \varphi \rrbracket_{\mathcal{J}[x \mapsto a]} = \mathbf{T}$
        \item $\llbracket \exists x \varphi \rrbracket_{\mathcal{J}} = \mathbf{T}$ if and only if for at least one $a$ in $\mathcal{A}$'s domain, $\llbracket \varphi \rrbracket_{\mathcal{J}[x \mapsto a]} = \mathbf{T}$
    \end{itemize}
    where $\mathcal{J}[x \mapsto a]$ is a $S$-interpretation which keeps all other interpretations in $\mathcal{J}$ and interprets $x$ by $a$.
\end{dy}

\begin{kuang3}
    \subsection{Quantiers with restricted domains}
\end{kuang3}

\subsubsection{The truth of "if-then"}

\begin{dl} \quad
    \begin{itemize}
        \item $\phi \rightarrow (\psi \rightarrow \phi) \equiv \mathbf{T}$.
        \item $(\phi \rightarrow \psi \rightarrow \chi) \rightarrow (\phi \rightarrow \psi) \rightarrow (\phi \rightarrow \chi) \equiv \mathbf{T}$.
        \item $\phi \rightarrow \psi \equiv \lnot \phi \lor \psi$
    \end{itemize}
\end{dl}

\begin{kuang1}
    \part{Discrete Math: Set Theory}
\end{kuang1}

\begin{kuang2}
    \section{The definition of set}
\end{kuang2}

(Omitted)

\begin{kuang2}
    \section{Relations}
\end{kuang2}

\begin{kuang3}
    \subsection{Relations}
\end{kuang3}

\subsubsection{Properties of relations}

\begin{dy}
    Given $R$, a relation on $A$, 
    \begin{itemize}
        \item \textbf{Reflexive} on $A$ if it holds that $\forall a \in A, (aRa) \Leftrightarrow I_A \subseteq R$
        \item \textbf{Symmetric} on $A$ if it holds that $\forall a, b \in A$ if $aRb$, then $bRa$ $\Leftrightarrow R^{-1} = R$
        \item \textbf{Transitive} on $A$ if it holds that $\forall a, b, c \in A$ if $aRb, bRc$, then $aRc$ $\Leftrightarrow R \circ R \subseteq R$
        \item \textbf{Antisymmetric} on $A$ if it holds that $\forall a, b \in A$ if $aRb, bRa$, then $a = b$ $\Leftrightarrow R \cap R^{-1} = I_A$
    \end{itemize}
\end{dy}

\subsubsection{Equivalence relations}

\begin{dy}
    If $R \subseteq A \times A$ is reflexive, symmetric and transitive, then $R$ is called a \textbf{equivalence relation} on $A$
\end{dy}

\begin{kuang3}
    \subsection{Relations and Sets}
\end{kuang3}

\subsubsection{Equivalence classes and Partitions}

\begin{dy}
    $R$ is an equivalence relation on $A$, $a \in A$, then we define the equivalence class $[a]_R$ of $A$ by
    \[
        [a]_R = \left\{b \in A | bRa \right\}
    \]
\end{dy}

\begin{dl}
    $aRb$ iff. $[a]_R = [b]_R$
\end{dl}

\subsubsection{Transitive Closures and Reflexive Transitive Closures}

\begin{dy}[Transitive Closures]
    Suppose $R$ is a relation on $A$, $R'$ is a transitive closure of $R$ if 
    \begin{itemize}
        \item $R \subseteq R'$
        \item $R'$ is transitive
        \item $\forall T$, $T$ is transitive, $R \subseteq T$, then $R' \subseteq T$. 
    \end{itemize}
    \begin{dyhj}[Another definition]
        $R^+ = \bigcup_{n = 1}^\infty R^n$ is the transitive closure 
    \end{dyhj}
\end{dy}

\begin{zm}
    Let's prove that the two definitions are equivalent. 
    \begin{itemize}
        \item $R \subseteq R^+$
        \item If $aR^+b, bR^+c$, then there exists $m, n$, $aR^mb$, $bR^nc$, then $aR^{m + n}c$, $R^+$ is transitive.
        \item If $R \subseteq T$ and $T$ is transitive, if $R^n \subseteq T$, then $R^{n + 1} = R^n \circ R \subseteq T \circ T \subseteq T$, so $R^+ = \bigcup_{n = 1}^\infty R^n \subseteq T$.
    \end{itemize}
    So such $R^+$ is a transitive closure.
\end{zm}

\begin{kuang2}
    \section{Functions}
\end{kuang2}

\begin{kuang3}
    \subsection{Functions}
\end{kuang3}

\begin{kuang3}
    \subsection{Funcions and Sets}
\end{kuang3}

\subsubsection{Injection and Surjection}

\begin{dy} \quad \\
    $F: A \to B$,
    \begin{itemize}
        \item \textbf{Injection}(one-to-one map): $\forall a, a' \in A$, if $F(a) = F(a')$, then $a = a'$.
        \item \textbf{Surjection}(onto map): $\forall b \in B, \exists a \in A, F(a) = b$.
        \item \textbf{Bijection}(one-to-one correspondence): both one-to-one and onto.
    \end{itemize}
\end{dy}

\begin{dl} \quad
    \begin{itemize}
        \item If $F, G$ are both injections, then $F \circ G$ is also an injection.
        \item If $F, G$ are both surjection, then $F \circ G$ is also a surjection.
        \item If $F \circ G$ is an injection, then $G$ is also an injection.
        \item If $F$ is an bijection, then $F^{-1}$ is also a bijection.
    \end{itemize}
\end{dl}

\begin{dl}[Berstern's Theorem]
    If there exist an injection from $A$ to $B$ and an injection from $B$ to $A$, then there exists a bijection between $A$ and $B$
\end{dl}

\begin{zm}
    Suppose $F$ is an one-to-one function from $A$ to $B$, $G$ is an one-to-one function from $B$ to $A$. \\
    Then we can construct a sequence of set as follow:
    \begin{align*}
        C_0 =& \left\{a \in A | \forall b \in B, G(b) \neq a\right\} = A \setminus \left\{a | \exists b \in B, G(b) = a\right\}, \\
        \quad D_0 =& \left\{F(a) | a \in C_0\right\} =B \setminus \left\{b \in B | \exists a \in A \setminus C_0 , b = F(a) \right\}
    \end{align*}
    $\forall n \geqslant 1$,
    \begin{align*}
        C_n =& \left\{a \in A \vert \forall b \in B \setminus \bigcup_{i = 0}^{n - 1}D_i, G(b) \neq a\right\} \\
        D_n =& \left\{F(a) \vert a \in C_n \right\} 
    \end{align*}
    Now we define a function $H$, where \\
    \[H(a) = \begin{cases}
        F(a), & \quad a \in \bigcup_{n = 0}^{\infty}C_n \\
        b\ (a = G(b)), & \quad a \notin \bigcup_{n = 0}^{\infty}C_n
    \end{cases}\]
    Let $C = A \setminus \bigcup_{n = 0}^{\infty}C_n$, $D = B \setminus \bigcup_{n = 0}^{\infty}D_n$ \\
    Now we prove that $H$ is well-defined and is a bijection.
    \begin{itemize}
        \item Firstly we prove that such $b$ exists. \\
        $\forall a \in C, a \notin C_0$, so $\exists b \in B$, $G(b) = a$. If $b \in D_n$, then $a = G(b) \in C_{n + 1}$, contradictive! So $b \in D$. Due to $G$ is an injection, such $b$ is unique.
        \item Then we prove that $H$ is an injection. \\
        $\forall a \in \bigcup_{n = 0}^{\infty}C_n, F(a) \in \bigcup_{n = 0}^{\infty}D_n$, and due to $F$ is an injection on $\bigcup_{n = 0}^{\infty}C_n$, $H$ is an injection. \\
        $\forall a \in C, \exists b \in D, a = G(b)$, due to $G$ is an injection on $C$, $H$ is an injection. 
        \item Finallty we prove that $H$ is a surjection. \\
        $\forall b \in \bigcup_{n = 0}^{\infty}D_n$ according to the define. \\
         $\forall b \in D, \exists a \in A, G(b) = a$, so $a \notin C_0$. If $a \in C_n (n \geqslant 1) $, then $b \in D_{n - 1}$, contradictive! So $a \in C$.
    \end{itemize}
\end{zm}

\subsubsection{Equinumerous Sets}

\begin{dy}\quad
    \begin{itemize}
        \item If there exists an injection from $A$ to $B$, then we write $A \preccurlyeq B$.
        \item If there exists a bijection between $A, B$, then we call $A, B$ are equinumerous, i.e. $A \approx B$ 
    \end{itemize}
\end{dy}

\begin{dy}
    Denote the set of function (or its cardinality) $\left\{F\ |\ F:\ A \to B\right\}$ by $B^A$
\end{dy}

\begin{dl}
    $\mathcal{P}(A) \approx \left\{F\ |\ F:\ A \to \left\{0, 1\right\}\right\}$
\end{dl}

\begin{zm}
    Let function $H:\ \mathcal{P}(A) \to \left\{F\ |\ F:\ A \to \left\{0, 1\right\}\right\}$, \\
    $\forall X \in \mathcal{P}(A), H(X)(a) = 1 \text{ iff. } a \in X$. \\
    For any $F \in \left\{F\ |\ F:\ A \to \left\{0, 1\right\}\right\}$, $X = \left\{a\ |\ F(a) = 1\right\} \in \mathcal{P}(A)$, $H(X) = F$.\\
    If $H(X_1) = H(X_2) = F$, then $X_1 = X_2 = \left\{a\ |\ F(a) = 1\right\}$.
\end{zm}

\begin{dl}
    If $A_1 \approx A_2, B_1 \approx B_2$, then $(A_1 \to B_1) \approx (A_2 \to B_2)$, i.e. $B_1^{A_1} \approx B_2^{A_2}$
\end{dl}

\begin{zm}
    There exist $f \in (A_1 \to A_2), g \in (B_1 \to B_2)$, $f, g$ are both bijections. \\
    Then let $H:\ (A_1 \to B_1) \to (A_2 \to B_2)$, for any $F: A_1 \to B_1$, $H(F) = g \circ F \circ f^{-1}$ \\
    $H(F_1) = H(F_2) \Rightarrow g \circ F_1 \circ f^{-1} = g \circ F_2 \circ f^{-1} \Rightarrow F_1 \circ f^{-1} = F_2 \circ f^{-1}$. According to $\forall b \in A_2, \exists a \in A_1, f(a) = b$. So $F_1 \circ f^{-1} = F_2 \circ f^{-1} \Rightarrow \forall b \in A_2, F_1 \circ f^{-1}(b) = F_2 \circ f^{-1}(b) \Rightarrow F_1(a) = F_2(a) \Rightarrow F_1 = F_2$. \\
    $\forall F_2 \in (A_2 \to B_2)$, let $F_1 = g^{-1} \circ F_2 \circ f$.
\end{zm}

\begin{dl}
    $(A \times B \to C) \approx (A \to (B \to C))$, i.e. $C^{A \times B} \approx \left(C^B\right)^A$
\end{dl}

\begin{zm}
    Let $H:\ (A \times B \to C) \to (A \to (B \to C))$, $H(F)(a)(b) = F(a, b)$. \\
    Omit the following proof.
\end{zm}

\begin{dl}[Cantor's Theorem]
    $\mathcal{P}(A)$'s cardinality is bigger than $A$'s.
\end{dl}

\begin{zm}
    Prove by contradiction. \\
    Assume that exists $A$, $\mathcal{P}(A) \approx A$, then there exists an bijection $\theta$ from $A$ to $\mathcal{P}(A)$. \\
    Let $X = \left\{x \in A\ |\ x \in \theta(x) \right\} \subseteq A$. \\
    Consider $x = \theta^{-1}(X)$. 
    \begin{itemize}
        \item If $x \in \theta(x) = X$, then according to the definition of $X$, $x \notin X$, impossiable! 
        \item If $x \notin \theta(x) = X$, then according to the definition of $X$, $x \in X$, impossiable!
    \end{itemize}
\end{zm}

\subsubsection{Countable Infinity and Uncountable Infinity}

\begin{lt}\quad
    \begin{itemize}
        \item $\NN$, $\NN \times \NN$, $\underbrace{\NN \times \cdots \times \NN}_{n \text{ times}}$ is countable.
        \item The set of all finit sequence of $\NN$ is countable. \\
        (equal to $\bigcup_{n = 1}^{+\infty}\underbrace{\NN \times \cdots \times \NN}_{n \text{ times}}$)
        \item $\QQ$ is countable. \\
        $\QQ \preccurlyeq \ZZ^+ \times \ZZ \approx \NN \times \NN \approx \NN$, $\NN \preccurlyeq \QQ$
    \end{itemize}
\end{lt}

\begin{lt}
    \begin{itemize}
        \item $2^{\NN} \approx \NN^{\NN}$
        \item $\RR \approx 2^{\NN}$
        \item $\RR^{\RR} \approx 2^{\RR} \approx \mathcal{P}(\RR)$
    \end{itemize}
\end{lt}

\begin{kuang3}
    \subsection{ZFC Set Theory}
\end{kuang3}

\subsubsection{The Definition of "="}

\begin{dy} Assembling a prelicate.
    \begin{itemize}
        \item (Axiom of reflexivity) $\forall x(x = x)$
        \item (Axiom of symmetry) (Omitted)
        \item (Axiom of transitivity) (Omitted)
        \item (Axiom of substitution) $\forall a \forall b (a = b \rightarrow (\phi[x \mapsto a] \rightarrow \phi[x \mapsto b]))$
    \end{itemize}
\end{dy}

\subsubsection{The Axioms of ZFC Set Theory}



\begin{dl}\quad
    \begin{itemize}
        \item (Axiom of Extension) $\forall A \forall B (A = B \Leftrightarrow \forall x (x \in A \leftrightarrow x \in B))$
        \item (Axiom of Union) $\forall \mathcal{A} \exists B \forall x (x \in B \leftrightarrow \exists C (C \in \mathcal{A} \land x \in C))$, we denote $B$ as $\bigcup \mathcal{A}$
        \item (Axiom of Power Set) $\forall A \exists \mathcal{B} \forall C(C \in \mathcal{B} \leftrightarrow C \subseteq A)$, we denote $\mathcal{B}$ as $\mathcal{P}(A)$
        \item (Axiom of Empty Set) $\exists X \forall x(\lnot x \in X)$, we denote such $X$ as $\varnothing$
        \item (Axiom of Infinity) $\exists X(\varnothing \in X \land \forall y(y \in X \rightarrow y \cup \{y\} \in X))$, we call such $X$ \textbf{inducive set}.
        \item (Axiom Schema of Specification) $\forall A \exists B \forall x (x \in B \leftrightarrow (x \in A \land \phi(x)))$, we denote such $B$ as $\left\{x \in A\ |\ \phi(x)\right\}$
        \item (Axiom of Regularity) $\forall A \exists y(y \in A \land y \cap A = \varnothing) \Leftrightarrow \forall A \exists y(y \in A \land \forall x (x \in A \rightarrow \lnot x \in y))$
    \end{itemize}
\end{dl}

\subsubsection{The Re-definition of Certain Concepts with ZFC}

\begin{dy}[The definition of nature numbers]\quad \\
    $0\ :\ \varnothing$ \\
    $1\ :\ 0 \cup \{0\}$ \\
    $2\ :\ 1 \cup \{1\}$ \\
    $\cdots$ \\
    We define $\NN$ as the smallest inducive set, i.e. for any inducive set $T$, $\NN \subseteq T$. \\
    Obviously all the numbers we defined w is the elements of $\NN$.
\end{dy}

\begin{dy}[The definition of ordered pairs]\quad \\
    We define $(a, b)$ as $\{\{a\}, \{a, b\}\}$.
\end{dy}

\begin{dy}[The options of nature numbers]
    The sum of $m, n \in \NN$ is $r$ iff. $(m, n, r) \in T$ where $T$ is the least set such that 
    \[
        \forall n,\quad (n, 0, n) \in T
    \]
    \[
        \forall n \forall m \forall r \left((n, m, r) \in T \rightarrow (n, m \cup \{m\}, r \cup \{r\}) \in T\right)
    \]
\end{dy}

\begin{dy}[Define transitive closures with ZFC]\label{Define transitive closures with ZFC}
    For any $R \subseteq A \times A$, we write $aR^nb$ iff. $(a, b, t) \in T$ where $T$ is the  least set such that 
    \[
        \forall a \forall b(aRb \rightarrow (a, b, 1) \in T)
    \]
    \[
        \forall n \forall a \forall b \forall c (aRb \land (b, c, n) \in T \rightarrow (a, c, n \cup \{n\}) \in T)
    \]
\end{dy}

\begin{dy}
    For any $R \subseteq A \times A$, $R^+ = \bigcup_{n \in \NN^+}R^n$ defines the following set according to the axiom of separating.
    \[
        \left\{(a, b) \in A \times A\ | \ \exists n ((a, b, n) \in T)\right\}
    \]
    where $T$ is the set defined in \textbf{Define\ref{Define transitive closures with ZFC}}.
\end{dy}

\begin{kuang3}
    \subsection{Inference Rules and Proof Theory}
\end{kuang3}

\begin{dy}[The natural deduction system] \quad \\
    $\Phi \vdash \psi$ iff. it can be established by the following proof rules in finite steps:
    \begin{itemize}
        \item $\phi[x \mapsto t] \vdash \forall x \phi$; $\forall x \phi \vdash \phi[x \mapsto t]$
        \item If $\Phi \vdash \psi$ and $x$ does not freely occur in $\Phi$, then $\Phi \vdash \forall x \psi$.
        \item If $\Phi, \psi \vdash \chi$ and $x$ does not freely occur in $\Phi$ or $\chi$, then $\Phi, \forall x\ \psi \vdash \chi$.
        \item $\phi, \psi \vdash \phi \land \psi$;\quad $\phi \land \psi \vdash \phi$;\quad $\phi \land \psi \vdash \psi$
        \item $\phi \vdash \phi \lor \psi$;\quad $\psi \vdash \phi \lor \psi$
        \item If $\Phi, \phi_1 \vdash \psi$ and $\Phi, \phi_2 \vdash \psi$, then $\Phi, \phi_1 \lor \phi_2 \vdash \psi$
        \item If $\Phi, \psi \vdash \chi$ and $\Phi, \neg \psi \vdash \chi$, then $\Phi \vdash \chi$
        \item If $\Phi, \neg \psi \vdash \chi$ and $\Phi, \neg \psi \vdash \neg \chi$, then $\Phi \vdash \psi$
        \item If $\phi \in \Phi$, then $\Phi \vdash \phi$
        \item If $\Phi \subseteq \Psi$ and $\Phi \vdash \phi$, then $\Psi \vdash \phi$
        \item If $\Phi \vdash \psi$ and $\Phi \vdash \psi \rightarrow \chi$, then $\Phi \vdash \chi$.
        \item If $\Phi, \psi \vdash \chi$, then $\Phi \vdash \psi \rightarrow \chi$.
    \end{itemize}
\end{dy}

\begin{dy}[Soundness]
    A first order logic (“$\vdash$”) is sound if $\Phi \vdash \psi$ implies $\Phi \models \psi$.
\end{dy}

\begin{dy}[Completeness]
    A first order logic (“$\vdash$”) is complete if $\Phi \models \psi$ implies $\Phi \vdash \psi$.
\end{dy}

\begin{kuang1}
    \part{Graph Theory}
\end{kuang1}

\begin{kuang2}
    \section{Graph in General}
\end{kuang2}

(Mostly omitted)

\begin{kuang3}
    \subsection{Basic definitions}
\end{kuang3}

\subsubsection{Edges and Degrees}

\begin{dy}[Adjacency and Incidence]
    \begin{itemize}
        \item     If  $ G = (V, E) $  is an undirected graph, two vertices  $ u, v \in V $  are adjacent (or neighbours) in  $ G $  if there is an edge  $ e \in E $  such that the endpoints of  $ e $  are  $ u, v $ . \\
        If the endpoints of an edge  $ e $  are  $ u, v $ , then  $ e $  is incident with  $ u, v $ .
        \item If  $ G = (V, E) $  is a directed graph and  $ e \in E $  is from  $ u $  to  $ v $ , then:  $ u $  is adjacent to  $ v $ , and  $ v $  is adjacent from  $ u $ ;  $ u $  is the initial vertex of the edge, while  $ v $  is the terminal (or end) vertex of the edge.
    \end{itemize}
\end{dy}

\begin{dy}[Neighbourhoods] \quad \\
    The neighbourhood  $ \mathcal{N}(v) $  is the set of all neighbours of  $ v $ . \\
    $ \mathcal{N}(A) := \bigcup_{v \in A} \mathcal{N}(v) $  for  $ A \subseteq V $ .
\end{dy}

\begin{dy}[Degrees]
    \begin{itemize}
        \item If  $ G = (V, E) $  is an undirected graph, the degree of a vertex  $ v \in V $  is the number of edges incident with it, for which a loop associated with  $ v $  contributes twice to the degree of  $ v $ . Notation: 
        \begin{align*}
            \deg(v) &= \left|\{e \mid v \text{ is } e\text{'s first endpoint}\}| + |\{e \mid v \text{ is } e\text{'s second endpoint}\}\right| \\
            &= \sum_{v \text{ is } e\text{'s first endpoint}} 1 + \sum_{v \text{ is } e\text{'s second endpoint}} 1 
        \end{align*} 
        \item If  $ G = (V, E) $  is a directed graph and  $ v \in V $ , we define:
        $$ \deg^{-}(v) := \left|\{e \in E \mid e \text{ is associated with } (u_1, v_1) \text{ and } v = v_1\}\right|\ \text{ (in-degree)}; $$ 
        $$ \deg^{+}(v) := \left|\{e \in E \mid e \text{ is associated with } (u_1, v_1) \text{ and } v = u_1\}\right|\ \text{ (out-degree)}. $$ 
    \end{itemize}
\end{dy}

\subsubsection{Loops and Circuits}

(Omitted)

\begin{kuang3}
    \subsection{Subgraph and Connected Components}
\end{kuang3}

\subsubsection{Connectivity of Undirected Graph}

\begin{dy}[Subgraph]
    (Omitted)
\end{dy}

\begin{dy}[Induced Subgraph]
    Suppose  $ G = (V, E) $  is a graph and  $ W \subseteq V $  is a subset of vertices. The subgraph induced by  $ W $  consists of all the vertices from  $ W $  and all the edges from  $ E $  whose endpoints both lie in  $ W $ .
\end{dy}

\begin{dy}[Connected Components]
    Suppose  $ G = (V, E) $  is an undirected graph. A connected component of  $ G $  is a connected subgraph that is not a proper subgraph of another connected subgraph of  $ G $ .
\end{dy}

\begin{dl}
    If  $ G $  is a nonempty undirected graph, then  $ G $ 's connected components are induced subgraphs of equivalence classes of the connectivity relation.
\end{dl}

\subsubsection{Reachability of Directed Graph}

\begin{dy}[Reachability]
    A vertex  $ v \in V $  is reachable from  $ u \in V $  if there is at least a path from  $ u $  to  $ v $  in  $ G $ . \\
    Two vertices  $ u, v \in V $  are mutually reachable if there are paths both from  $ u $  to  $ v $  and from  $ v $  to  $ u $  in  $ G $ . \\
    If $u, v \in V$ are mutually reachable, then we call $u$ and $v$ are strongly connected.
\end{dy}

\begin{dy}[Strongly-Connected Components]
    Suppose  $ G = (V, E) $  is a directed graph. A strongly-connected component of  $ G $  is a strongly-connected subgraph of  $ G $  that is not a proper subgraph of another strongly-connected subgraph of  $ G $ .
\end{dy}

\begin{dl}
    Given a directed graph  $ G $ , mutual reachability in  $ G $  is an equivalence relation. \\
    Given a nonempty directed graph  $ G $ , its strongly-connected components are induced subgraphs of equivalence classes of mutual reachability.
\end{dl}

\subsubsection{Connectivity against Vertices and Edges Removal}

(Omitted)

\begin{kuang2}
    \section{Tree}
\end{kuang2}

\begin{kuang3}
    \subsection{Unrooted tree}
\end{kuang3}

\begin{dy}[Trees]
    A tree is a connected (nonempty) undirected graph without simple circuits.
\end{dy}

\begin{dy}[Leaves (in an unrooted tree)]
    A vertex is a leaf in a tree if its degree is 1.
\end{dy}

\begin{dl}
    All statements below about an undirected graph $G = (V,E)$ are equivalent:
    \begin{itemize}
        \item $G$ is a tree, i.e. $G$ is connected but contains no simple circuits.
        \item $G$ is connected and $|E| = |V| - 1$
        \item $G$ contains no simple circuits and $|E| = |V| - 1$
        \item $G$ is connected, but every edge in $E$ is a cut edge.
        \item $G$ contains no simple circuits, adding any edge to $G$ generates a simple circuit.
        \item There is a unique simple path between any two $G$'s vertices.
    \end{itemize}
\end{dl}

\begin{kuang3}
    \subsection{Rooted tree}
\end{kuang3}

\begin{dy}[Rooted trees]
    A rooted tree is a tree with a designated vertex (as the root)
\end{dy}

\begin{dy}[Levels]
    If  $ G = (V, E) $  is a rooted tree with the root  $ r $ , we define that:
    \begin{itemize}
        \item the level of a vertex  $ v $  is the length of the unique simple path from  $ r $  to  $ v $ ;
        \item the height of the tree is the maximal level of its vertices.
    \end{itemize}
\end{dy}
    
\begin{dy}[Parents and Children]
    If  $ G = (V, E) $  is a rooted tree with the root  $ r $ , the parent of a vertex  $ v \neq r $  is the unique vertex  $ u $  such that  $ (u, v) \in E $  and this edge appears on the unique simple path between  $ r $  and  $ v $ . Also,  $ v $  is called a child of  $ u $ .
\end{dy}
    
\begin{dy}[Siblings]
    If  $ G = (V, E) $  is a rooted tree with the root  $ r $ , vertices  $ u $  and  $ v $  are siblings if they have the same parent.
\end{dy}
    
\begin{dy}[Ancestors and Descendants]
    If  $ G = (V, E) $  is a rooted tree with the root  $ r $ , the ancestors of a vertex  $ v \neq r $  are the vertices on the simple path from  $ r $  to  $ v $ , excluding  $ v $  but including  $ r $ , and the descendants of a vertex  $ v $  are all vertices that have  $ v $  as one of their ancestors.
\end{dy}

\begin{dy}[Subtree]
    If  $ G = (V, E) $  is a rooted tree with the root  $ r $ , the subtree at a vertex  $ v $  is the induced subgraph of the vertex set consisting of the vertex  $ v $  (as its root) and all the descendants of  $ v $ .
\end{dy}

\begin{kuang2}
    \section{Spanning tree, Eular path and Hamilton paths}
\end{kuang2}

\begin{kuang3}
    \subsection{Spanning tree}
\end{kuang3}

\subsubsection{Spanning tree}


\begin{dy}[Spanning Trees]
    Suppose  $ G $  is an undirected graph. A spanning tree of  $ G $  is a subgraph of  $ G $  that is a tree containing every vertex of  $ G $ .
\end{dy}
    
\begin{dl}
    An undirected graph is connected if and only if it has a spanning tree.
    \begin{zmhj} \quad
        \begin{itemize}
            \item If a spanning tree exists, then there is a path in the spanning tree between any two vertices. Thus the graph is also connected.
            \item Suppose  $ G_0 = G $  is connected. If  $ G_0 $  contains a simple circuit, then removing one edge from the simple circuit, which generates graph  $ G_1 $ .  $ G_1 $  must be connected. Repeat this process and construct  $ G_2, G_3, \cdots $ . In this process, the number of edges keep decreasing. Thus, there must be a natural number  $ k $  such that the number of vertices in  $ G_k $  is one more than its edges. That must be a tree.
        \end{itemize}
    \end{zmhj}
\end{dl}

\subsubsection{Minimum spanning tree}

\begin{dy}[Minimum spanning tree]
    A minimalspanning tree of $G$ is a spanning tree whose sum of all weights in the tree is the minimum among all spanning trees.
\end{dy}

\subsubsection{Algorithms to construct minimum spanning tree}

(Omitted)

\begin{kuang3}
    \subsection{Eular paths and circuits}
\end{kuang3}

\begin{dy}
    Given $G = (V, E)$ is a graph.
    \begin{itemize}
        \item an Euler circuit in $G$ is a simple circuit containing every edge of $G$.
        \item an Euler path in $G$ is a simple path containing every edge of $G$.
    \end{itemize}
\end{dy}

\begin{dl}
    A connected undirected graph with at least two vertices has an Euler circuit if and only if all of its vertices have even degree.
    \begin{zmhj}
        By induction on the number of edges.
        \begin{itemize}
            \item \textbf{Base Step:} two edges
            \item \textbf{Inductive Step:}
            \begin{itemize}
                \item A simple path of maximal length is a circuit, or otherwise the parity of the degrees at the start and end does not match.
                \item A simple circuit of maximal length is an Euler circuit, or otherwise we get an undirected multigraph whose vertices have even degree when we remove the circuit, from which we can construct an Euler circuit in a connected component that can be merged back to the original one.
            \end{itemize}
        \end{itemize}
    \end{zmhj}
\end{dl}

\begin{kuang3}
    \subsection{Hamilton paths and circuits}
\end{kuang3}

\begin{dy}[Hamilton Paths and Circuits]
    Given an undirected graph  $ G = (V, E) $ ,
    \begin{itemize}
        \item a Hamilton path is a simple path  $ v_0, v_1, \cdots, v_n $  of distinct vertices in  $ G $  such that  $ V = \{v_0, v_1, \cdots, v_n\} $ ;
        \item a Hamilton circuit is a simple circuit  $ v_0, v_1, \cdots, v_n, v_0 $  ( $ n \geq 0 $ ) such that  $ V = \{v_0, v_1, \cdots, v_n\} $  and  $ v_0, v_1, \cdots, v_n $  is a Hamilton path.
    \end{itemize}
\end{dy}

\begin{kuang1}
    \part{Counting Theory}
\end{kuang1}

\begin{kuang2}
    \section{Counting Theory}
\end{kuang2}

\begin{kuang3}
    \subsection{Inclusion-Exclusion Principle}
\end{kuang3}

\begin{dl}[Inclusion-Exclusion Principle]
    If  $ A_1, \cdots, A_n $  are finite sets, then
    \begin{align*}
        \left| \bigcup_{i=1}^n A_i \right| = \sum_{\ell=1}^n (-1)^{\ell+1} \sum_{1 \leqslant k_1 < \cdots < k_\ell \leqslant n} \left| \bigcap_{j=1}^\ell A_{k_j} \right|
    \end{align*}
\end{dl}



\end{document}